theories/iris/language/cwp/structural.v
@@ -1,3 +1,5 @@
+Require Import stdpp.base.
+
 Require Import iris.proofmode.tactics.
 
 Require Import RichWasm.iris.helpers.prelude.iris_wasm_lang_properties.
@@ -11,6 +13,59 @@ Section structural.
 
   Context `{!wasmG Σ}.
 
+  Lemma has_values_iff_map_const es vs :
+    has_values es vs <-> es = map BI_const vs.
+  Proof.
+    split.
+    {
+      generalize dependent vs. induction es.
+      - intros vs H.
+        apply Is_true_true in H.
+        apply all2_size in H.
+        symmetry in H.
+        apply seq.size0nil in H.
+        by rewrite H.
+      - intros vs H. destruct vs.
+        + apply Is_true_true in H. apply all2_size in H. inversion H.
+        + cbn in H.
+          apply andb_True in H as [Hv Hvs].
+          apply IHes in Hvs.
+          subst es.
+          rewrite map_cons.
+          destruct a; try inversion Hv.
+          cbn in Hv.
+          destruct (value_eq_dec v v0) as [-> | Hv0] eqn:Heq; first done.
+          unfold value_eqb in Hv.
+          by rewrite Heq in Hv.
+    }
+    {
+      generalize dependent vs. induction es.
+      - intros vs H. symmetry in H. apply map_eq_nil in H. by subst vs.
+      - intros vs H. destruct vs.
+        + inversion H.
+        + rewrite map_cons in H.
+          inversion H.
+          apply IHes in H2.
+          subst a.
+          cbn.
+          apply andb_True.
+          split.
+          * unfold value_eqb. by destruct (value_eq_dec v v).
+          * inversion H. by rewrite <- H1.
+    }
+  Qed.
+
+  Lemma has_values_consts vs :
+    has_values (to_consts vs) vs.
+  Proof.
+    induction vs; first done.
+    cbn.
+    apply andb_True.
+    split.
+    - unfold value_eqb. by destruct (value_eq_dec a a).
+    - apply IHvs.
+  Qed.
+
   Lemma cwp_nil s E (f : frame) L R Φ :
     ↪[frame] f -∗ ↪[RUN] -∗ Φ f [] -∗ CWP [] @ s; E UNDER L; R {{ Φ }}.
   Proof.
@@ -19,10 +74,14 @@ Section structural.
     iFrame.
   Qed.
 
-  Lemma cwp_val s E f vs L R Φ :
-    ↪[frame] f -∗ ↪[RUN] -∗ Φ f vs -∗ CWP (map BI_const vs) @ s; E UNDER L; R {{ Φ }}.
+  Lemma cwp_val s E f vs evs L R Φ :
+    has_values evs vs ->
+    ↪[frame] f -∗
+    ↪[RUN] -∗
+    Φ f vs -∗
+    CWP evs @ s; E UNDER L; R {{ Φ }}.
   Proof.
-    iIntros "Hf Hrun HΦ".
+    iIntros (Hevs) "Hf Hrun HΦ".
     iApply lenient_wp_value.
     - instantiate (1 := immV vs).
       unfold IntoVal.
@@ -30,15 +89,20 @@ Section structural.
       unfold v_to_e_list, to_e_list.
       change (@seq.map value _) with (@map value administrative_instruction).
       change (@seq.map basic_instruction _) with (@map basic_instruction administrative_instruction).
+      apply has_values_iff_map_const in Hevs.
+      subst evs.
       by rewrite map_map.
     - iFrame.
   Qed.
 
-  Lemma cwp_val_app E vs es L R Φ :
+  Lemma cwp_val_app E vs evs es L R Φ :
+    has_values evs vs ->
     CWP es @ E UNDER L; R {{ fvs_combine Φ vs }} -∗
-    CWP (map BI_const vs ++ es) @ E UNDER L; R {{ Φ }}.
+    CWP evs ++ es @ E UNDER L; R {{ Φ }}.
   Proof.
-    iIntros "Hes".
+    iIntros (Hevs) "Hes".
+    apply has_values_iff_map_const in Hevs.
+    subst evs.
     unfold cwp_wasm, to_e_list.
     change seq.map with (@map basic_instruction administrative_instruction).
     rewrite map_app.
@@ -99,7 +163,7 @@ Section structural.
     CWP es1 @ E UNDER L; R {{ Φ1 }} -∗
     (∀ f vs,
      Φ1 f vs -∗ ↪[frame] f -∗ ↪[RUN] -∗
-     CWP map BI_const vs ++ es2 @ s; E UNDER L; R {{ Φ2 }}) -∗
+     CWP to_consts vs ++ es2 @ s; E UNDER L; R {{ Φ2 }}) -∗
     CWP es1 ++ es2 @ s; E UNDER L; R {{ Φ2 }}.
   Proof.
     iIntros "Hes1 Hes2".
